src/proof/text/Observe.v
@@ -71,10 +71,10 @@ Proof.
   subst text_store parent.
   wp_auto.
   wp_apply (wp_Store__wlock with "[$His_store]"). iIntros "[Hlk Hinv]".
-  iDestruct "Hinv" as (c h m pend deleted) "[Hstore Hreg]".
+  iDestruct "Hinv" as (c h m pend deleted observers_mref) "[Hstore Hreg]".
   wp_auto.
   (* ---- the current text ---- *)
-  iDestruct "Hstore" as (client k pdel locs p bind acc) "Hown". iNamed "Hown".
+  iDestruct "Hstore" as (client k pdel locs p bind acc observers_mref0) "Hown". iNamed "Hown".
   iDestruct (ghost_map_lookup with "HtypesAuth Hbind") as %Hbindlk.
   iDestruct (own_store_state_registry_coh with "Hstate") as %Hregcoh.
   iDestruct (own_store_state_run_pool_invs with "Hstate") as %Hpoolinv.
@@ -108,10 +108,12 @@ Proof.
     destruct (run_per_char_content (run_items r) x (Hperchar r Hr) Hxitems) as [b Hb].
     rewrite Hb. discriminate. }
   iNamed "Hreg".
+  (* the registry's map is the store's [observers] field *)
+  iDestruct (is_store_observers_agree with "Hobserverspin Hregistrypin") as %Heqref. subst observers_mref0.
   iDestruct (registered_bindings_lookup with "HtypesAuth Hregistered_bind") as %Hregbind.
   iAssert (own_store tv.(yjs.Text.store') γs γh c h m pend deleted)
-    with "[Hstate Hseq HtypesAuth Hhist Hacc Hdelete_set]" as "Hstore".
-  { iExists client, k, pdel, locs, p, bind, acc. iFrame "∗#". iPureIntro. split_and!;
+    with "[Hstate Hseq HtypesAuth Hhist Hacc Hdelete_set Hobserversf]" as "Hstore".
+  { iExists client, k, pdel, locs, p, bind, acc, observers_mref. iFrame "∗#". iPureIntro. split_and!;
       [exact Hclientc | exact Hpendroot | exact Hpendbnd | exact Hregmodel | exact Hhcoh
       | exact Hctr | exact Hacccoh | exact Hdeleted]. }
   iMod (own_store_text_snapshot with "Hbind Hstore") as "[Hstore #Hsnapshot]".
@@ -149,9 +151,11 @@ Proof.
   wp_apply ("Hcb" $! initial_sl (DfracOwn 1) [] (type_snapshot m deleted name) with "[Hobs Hdelta]").
   { iFrame "Hobs Hdelta Hsnapshot". iPureIntro. apply snapshot_grows_to_nil. }
   iIntros "[Hobs Hdelta]".
-  wp_auto.
   (* ---- the registration: the type's callback slice grows by [cb], the
-     authority by the token ---- *)
+     authority by the token; the [observers] field is read off the store ---- *)
+  iDestruct (own_store_observers_acc with "Hstore") as (observers_mref1) "(#Hpin1 & Hobserversf & Hstoreback)".
+  iDestruct (is_store_observers_agree with "Hpin1 Hregistrypin") as %Heqref1. subst observers_mref1.
+  wp_auto.
   wp_apply (wp_map_lookup1 with "Hobserversmap"). iIntros "Hobserversmap".
   wp_auto.
   iDestruct (big_sepM2_dom with "Hobservers") as %Hdomeq.
@@ -169,11 +173,12 @@ Proof.
     wp_apply (wp_slice_append with "[$Hentry_slice $Hentry_cap $Hs2]").
     iIntros (sl') "(Hsl' & Hcap' & _)". wp_auto.
     wp_apply (wp_map_insert with "Hobserversmap"). iIntros "Hobserversmap". wp_auto.
+    iDestruct ("Hstoreback" with "Hobserversf") as "Hstore".
     iMod (observers_register γs _ γo name with "Hobserversauth") as "[Hobserversauth #Hobserved]".
-    wp_apply (wp_Store__wunlock with "[$His_store $Hlk $Hstore Hobserversf Hobserversmap Hobserversauth Hobservers Hsl' Hcap' Hentry_callbacks Hobs]").
-    { iExists observers_mref, (<[tv.(yjs.Text.inner') := sl']> registry),
+    wp_apply (wp_Store__wunlock with "[$His_store $Hlk $Hstore Hobserversmap Hobserversauth Hobservers Hsl' Hcap' Hentry_callbacks Hobs]").
+    { iExists (<[tv.(yjs.Text.inner') := sl']> registry),
         (<[tv.(yjs.Text.inner') := (name, γos ++ [γo])]> registered).
-      iFrame "Hobserversf Hobserversmap".
+      iFrame "Hregistrypin Hobserversmap".
       rewrite (registered_tokens_register registered _ name γos γo (or_introl Hdkey)).
       iFrame "Hobserversauth".
       iSplitR.
@@ -190,11 +195,12 @@ Proof.
     { iSplitR; [iApply own_slice_nil | iSplitR; [iApply own_slice_cap_nil | iFrame "Hs2"]]. }
     iIntros (sl') "(Hsl' & Hcap' & _)". wp_auto.
     wp_apply (wp_map_insert with "Hobserversmap"). iIntros "Hobserversmap". wp_auto.
+    iDestruct ("Hstoreback" with "Hobserversf") as "Hstore".
     iMod (observers_register γs _ γo name with "Hobserversauth") as "[Hobserversauth #Hobserved]".
-    wp_apply (wp_Store__wunlock with "[$His_store $Hlk $Hstore Hobserversf Hobserversmap Hobserversauth Hobservers Hsl' Hcap' Hobs]").
-    { iExists observers_mref, (<[tv.(yjs.Text.inner') := sl']> registry),
+    wp_apply (wp_Store__wunlock with "[$His_store $Hlk $Hstore Hobserversmap Hobserversauth Hobservers Hsl' Hcap' Hobs]").
+    { iExists (<[tv.(yjs.Text.inner') := sl']> registry),
         (<[tv.(yjs.Text.inner') := (name, [] ++ [γo])]> registered).
-      iFrame "Hobserversf Hobserversmap".
+      iFrame "Hregistrypin Hobserversmap".
       rewrite (registered_tokens_register registered _ name [] γo (or_intror (conj Hdkey eq_refl))).
       iFrame "Hobserversauth".
       iSplitR.
